filter.v
@@ -1,0 +1,50 @@
+Require Import ZArith.
+Require Import List.
+Require Import Bool.
+Import ListNotations.
+Open Scope Z_scope.
+
+Fixpoint solution (pred:Z -> bool) (lst:list Z) : list Z :=
+    match lst with
+    | [] => []
+    | hd::tl => if pred hd then hd :: solution pred tl else solution pred tl
+    end.
+
+Definition filter_sub (pred:Z -> bool) (lst: list Z) : list Z :=
+    let fix aux (i:Z) (l :list Z) : list Z :=
+    match l with
+    | [] => []
+    | hd::tl => if pred hd then hd:: aux (i+1) tl else aux(i+1) tl
+    end in
+    aux 1 lst.
+  
+Lemma list_eq_tail : forall (a : nat) (b c : list nat),
+  a :: b = a :: c -> b = c.
+Proof.
+  intros a b c H.
+  injection H as H1.
+  exact H1.
+Qed.
+
+
+
+
+
+
+
+Theorem eq : forall pred lst, solution pred lst = filter_sub pred lst.
+Proof.
+    intros.
+    unfold filter_sub.
+    induction lst.
+    simpl.
+    reflexivity.
+    simpl.
+    case (pred a).
+    rewrite IHlst.
+    
+    Search (_::_ ).
+
+    
+    
+    
