formula.v
@@ -1,22 +1,26 @@
 Require Import ZArith.
+Require Import Recdef.
+Require Import Bool.
+Open Scope Z_scope.
+
 Inductive exp : Type :=
 | Num : Z -> exp
-| Plus : (exp*exp) -> exp
-| Minus : (exp * exp) -> exp.
+| Plus : exp -> exp -> exp
+| Minus : exp -> exp -> exp.
 Inductive formula : Type :=
 | _True
 | _False
 | Not : formula -> formula
-| AndAlso : (formula * formula) -> formula
-| OrElse : (formula * formula) -> formula
-| Imply : (formula * formula) -> formula
-| Equal : (exp * exp) -> formula.
+| AndAlso : formula -> formula -> formula
+| OrElse : formula -> formula -> formula
+| Imply : formula -> formula -> formula
+| Equal : exp -> exp -> formula.
 
 Fixpoint exp_eval (exp:exp) : Z :=
 match exp with
 | Num n => n
-| Plus (e1, e2) => (exp_eval e1) + (exp_eval e2)
-| Minus (e1, e2) => (exp_eval e1) - (exp_eval e2)
+| Plus e1 e2 => (exp_eval e1) + (exp_eval e2)
+| Minus e1 e2 => (exp_eval e1) - (exp_eval e2)
 end.
 
 
@@ -25,8 +29,29 @@ match f with
 | _True => true
 | _False => false
 | Not f => negb (eval f)
-| AndAlso (f1, f2) => (eval f1) && (eval f2)
-| OrElse (f1, f2) => (eval f1) || (eval f2)
-| Imply (f1, f2) => (negb (eval f1)) || (eval f2)
-| Equal (e1, e2) => Z.eqb (exp_eval e1)  (exp_eval e2)
+| AndAlso f1 f2 => (eval f1) && (eval f2)
+| OrElse f1 f2 => (eval f1) || (eval f2)
+| Imply f1 f2 => (negb (eval f1)) || (eval f2)
+| Equal e1 e2 => Z.eqb (exp_eval e1)  (exp_eval e2)
 end.
+
+Fixpoint evall (exp:exp) : Z :=
+match exp with
+| Num a => a
+| Plus a b => evall(a)+evall(b)
+| Minus a b => evall(a)-evall(b)
+end.
+
+Fixpoint eval_sub (f : formula) : bool :=
+  match f with
+  | _True => true
+  | _False => false
+  | Not a => if (eval_sub a) then false else true
+  | AndAlso a b => (eval_sub a) && (eval_sub b)
+  | OrElse a b => (eval_sub a) || (eval_sub b)
+  | Imply a b => eval_sub (Not (AndAlso a (Not b)))
+  | Equal a b => if (Z.eqb (evall a) (evall b)) then true else false
+  end.
+    
+    
+       
